MasterThesis/Compiler/Compiler_v1.lean
@@ -1,11 +1,32 @@
+/-
+"A Lean-certified reversibilization of Meyer-Ritchie LOOP language".
+Master thesis in computer science, University of Turin.
+Authors: Andrea Delmastro
+-/
 import MasterThesis.SCORE.Language
 import MasterThesis.LOOP.Language
+
+/-!
+# Compiler for LOOP language, version 1
+
+This file defines a compiler that translates (_reversibilizes_) any LOOP program into a corresponding
+SCORE program based on a specific notion of equivalence between LOOP states and SCORE states.
+
+## Notations
+
+* `s ∼ t` stands for `eq_states s t` (`s` _and_ `t` _are equivalent_).
+-/
 
 namespace Compiler
 
 open LOOP Com
 open SCORE Com
 
+namespace v1
+
+/-- Syntax-directed compiler from LOOP programs to SCORE programs. The compiler takes as input a
+`LOOP.Com` and outputs the equivalent `SCORE.Com`.
+-/
 def l2s (P : LOOP.Com) : SCORE.Com :=
   match P with
   | .SKIP     => SKIP
@@ -18,5 +39,84 @@ def l2s (P : LOOP.Com) : SCORE.Com :=
   | .SEQ P Q  => l2s P;;
                  l2s Q
   | .LOOP x P => FOR x (l2s P)
+
+end v1
+
+open v1
+
+/-- Notion of equivalence between LOOP states and SCORE states. A LOOP state `s` is said to be
+equivalent to a SCORE state `t` if for each identifier `x` the value of the register identified
+by `x` in `s` is equal to the current value of the variable identified by `x` in `t`. -/
+def eq_states (s : LOOP.State) (t : SCORE.State) : Prop :=
+  match s, t with
+  | some σ, some τ => ∀ (x : Ident), some ↑(σ x) = (τ x).head?
+  | _     , _      => False
+
+infix:50 "∼" => eq_states
+
+/-- Two states are kept equivalent if the first is updated by assigning a new value `v` to the
+register identified by `x` and the second is updated by inserting `v` on top of the stack identified
+by `x`. -/
+lemma eq_states_update {σ : LOOP.Store} {τ : SCORE.Store} (x : Ident) (v : ℕ) : σ ∼ τ → σ[x ↦ v] ∼ τ[x ↦ ↑v :: τ x] := by
+  intros _ y
+  cases eq_or_ne x y
+  · simp [‹x = y›]
+  · simpa [‹x ≠ y›] using ‹σ ∼ τ› y
+
+/-- Evaluating the SCORE command `INC x` is equivalent to incrementing its current value by one in a
+LOOP state.  -/
+lemma eq_states_INC {σ : LOOP.Store} {t : SCORE.State} {x : Ident} {v : ℕ} : σ[x ↦ v] ∼ t → σ[x ↦ v + 1] ∼ SCORE.eval (.INC x) t := by
+  intro
+  cases t
+  case some τ _ =>
+    rw [SCORE.eval]
+    simp only [←‹σ[x ↦ v] ∼ τ› x]
+    intro y
+    cases eq_or_ne x y
+    · simp [‹x = y›]
+    · simpa [‹x ≠ y›] using ‹σ[x ↦ v] ∼ τ› y
+  case none =>
+    contradiction
+
+/-- Let `P` be a LOOP program, `σ` a LOOP state and `τ` a SCORE state. If the two states are equivalent,
+then the evaluation of `P` in `σ` and the compiled SCORE program `l2s P` in `τ` end in two equivalent
+states. -/
+theorem soundness {s : LOOP.State} {t : SCORE.State} (P : LOOP.Com) : s ∼ t → (LOOP.eval P s) ∼ (SCORE.eval (l2s P) t) := by
+  intro eqs
+  induction P generalizing s t
+  all_goals (cases s <;> cases t)
+  case SKIP.some.some σ τ =>
+    rwa [LOOP.eval, l2s, SCORE.eval]
+  case ZER.some.some x σ τ =>
+    rw [LOOP.eval, l2s, SCORE.eval]
+    exact eq_states_update x 0 ‹σ ∼ τ›
+  case ASN.some.some x y σ τ =>
+    rw [LOOP.eval]
+    cases eq_or_ne x y
+    · simpa [l2s, ‹x = y›, SCORE.eval]
+    · have : SCORE.eval (l2s (.ASN x y)) τ = (fun τ ↦ SCORE.eval (.INC x) τ)^[σ y] (τ[x ↦ 0 :: τ x]) := by
+        simp [l2s, ‹x ≠ y›, SCORE.eval, ←(‹σ ∼ τ› y)]
+      rw [this]; clear this
+      induction (σ y)
+      case zero =>
+        simpa using eq_states_update x 0 ‹σ ∼ τ›
+      case succ m ih =>
+        simpa [Nat.add_comm m 1, Function.iterate_add_apply] using eq_states_INC ih
+  case INC.some.some x σ τ =>
+    rw [LOOP.eval, l2s]
+    rw [←@LOOP.Store.update_no_update σ x] at ‹σ ∼ τ›
+    exact eq_states_INC ‹σ[x ↦ σ x] ∼ τ›
+  case SEQ.some.some Q R ih₁ ih₂ σ τ =>
+    rw [LOOP.eval, l2s, SCORE.eval]
+    exact ih₂ (ih₁ ‹σ ∼ τ›)
+  case LOOP.some.some x Q ih σ τ =>
+    simp [LOOP.eval, l2s, SCORE.eval, ←(‹σ ∼ τ› x)]
+    generalize some σ = s, some τ = t at ‹σ ∼ τ›
+    induction σ x generalizing s t
+    case zero =>
+      simpa
+    case succ _ ih₂ =>
+      exact ih₂ (LOOP.eval Q s) (SCORE.eval (l2s Q) t) (ih ‹s ∼ t›)
+  all_goals (simp only [eq_states] at eqs)
 
 end Compiler
