MasterThesis.lean
@@ -4,5 +4,4 @@ import MasterThesis.LOOP.Language
 import MasterThesis.LOOP.Parser
 import MasterThesis.Compiler.Compiler_v1
 --import MasterThesis.Compiler.Compiler_v2
-import MasterThesis.Compiler.Proofs.Compiler_v1
 --import MasterThesis.Compiler.Proofs.Compiler_v2
