MasterThesis/Compiler/Proofs/Commons.lean
@@ -3,23 +3,4 @@ import MasterThesis.LOOP.Language
 import MasterThesis.SCORE.Language
 import MasterThesis.Compiler.Commons
 
-lemma eq_states_update {σ : LOOP.Store} {τ : SCORE.Store} (x : Ident) (v : ℕ) : σ ∼ τ → σ[x ↦ v] ∼ τ[x ↦ ↑v :: τ x] := by
-  intros _ y
-  cases eq_or_ne x y
-  · simp [‹x = y›]
-  · simpa [‹x ≠ y›] using ‹σ ∼ τ› y
-
-lemma eq_states_INC {σ : LOOP.Store} {t : SCORE.State} {x : Ident} {v : ℕ} : σ[x ↦ v] ∼ t → σ[x ↦ v + 1] ∼ SCORE.eval (.INC x) t := by
-  intro
-  cases t
-  case some τ _ =>
-    rw [SCORE.eval]
-    simp only [←‹σ[x ↦ v] ∼ τ› x]
-    intro y
-    cases eq_or_ne x y
-    · simp [‹x = y›]
-    · simpa [‹x ≠ y›] using ‹σ[x ↦ v] ∼ τ› y
-  case none =>
-    contradiction
-
 lemma eq_states_idents_subs {s : LOOP.State} {t : SCORE.State} {a b : Finset Ident} : s =[a ∪ b]ₛ t → s =[a]ₛ t := by sorry
